%%%%%%%%%%%%%%%%%%%%%%%%%%%%%%%%%%%%%%%%%%%%%%%%%%%%%%%%%%%%%%%%
% Welcome to Overleaf --- just edit your LaTeX on the left,
% and we'll compile it for you on the right. If you open the
% 'Share' menu, you can invite other users to edit at the same
% time. See www.overleaf.com/learn for more info. Enjoy!
%
%%%%%%%%%%%%%%%%%%%%%%%%%%%%%%%%%%%%%%%%%%%%%%%%%%%%%%%%%%%%%%%

% Inbuilt themes in beamer
\documentclass{beamer}

% Theme choice:
\usetheme{CambridgeUS}
\usepackage{amsmath}
\usepackage{derivative}
\providecommand{\pr}[1]{\ensuremath{\Pr\left(#1\right)}}

% Title page details: 
\title{Assignment 5} 
\author{maloth david (CS21BTECH11035)}
\date{\ June 14}

\begin{document}

% Title page frame
\begin{frame}
    \titlepage 
\end{frame}

% Outline frame
\begin{frame}{Outline}
    \tableofcontents
\end{frame}


% Lists frame
\section{Problem}
\begin{frame}{Problem Statement}

\textbf{(Papoulis chapter 9 ,ex 9.29 )} find $E\{y^2(t)\}$ a) If  $R_X_X(\tau) =5\delta(\tau)$ and y'(t)+2y(t) = X(t) all t. b) if i) holds for  t \textgreater 0 only and y(t)= 0 for  t $\leq$ 0

\end{frame}


% Blocks frame
\section{Solution}
\begin{frame}{Solution}

\begin{itemize}

\item a) if y'(t)+2y(t) = X(t), then y(t) =x(t)*h(t)
\item where h(t) = ${e^{-2t}}u(t)$ and with q(t)=5, (10-90) yields
\item $E\{y^2(t)\}$ = 5*${e^{-4t}}U(T)$=5*$\int_0^\infty{e^{-4t}}d(\tau)$ =$\dfrac{5}{4}$
\item b) as a) with q(t) = 5U(t).hence,for t \textgreater 0
 
\item $E\{y^2(t)\}$ = $5U(t)*{e^{-4t}U(t)}$ =$5*\int_0^t{e^{-4t}d\tau}$ =$ \dfrac{5}{4}(1-{e^{-4t}}) $
\item hence proved
\end{itemize}
    
    
\end{frame} 



\end{document}
Â© 2022 GitHub, Inc.
Terms
Privacy
Security
Status
Docs
Co